com.io7m.medrina.documentation/src/main/coq/Medrina/Actions.v
@@ -72,3 +72,4 @@ Instance actionNameName : IsValidName actionName := {
 Record action : Set := AMake {
   aName : actionName
 }.
+
